\documentclass{ximera}

\input{../preamble.tex}


\outcome{Identify separable differential equation.}
\outcome{Compute general solution of a separable differential equation.}
\outcome{Find implicit solutions of a separable differential equation.}

\title[Dig-In:]{Separable differential equations}

\begin{document}
\begin{abstract}
  Separable differential equations are those in which the dependent and independent variables can be separated on opposite sides of the equation.
\end{abstract}
\maketitle

In this section we will see that the phrase
\begin{quote}
  Divide and Conquor
\end{quote}
is literally true (with the mathematical definition of ``divide'') in
the context of differential equations. Rather than talk about math,
let's just show you what we're getting at.

\begin{example}
  Solve the differential equation
  \[
  y'(x) = x\cdot y(x)^2
  \]
  where $y(0)= 5$.
  \begin{explanation}
    We're going to divide an conqur, literally. Divide both sides of
    \[
    y'(x) = x\cdot y(x)^2
    \]
    by $y(x)^2$ to find
    \[
    \frac{y'(x)}{y(x)^2} = \answer[given]{x}.
    \]
    Now integrate both sides with respect to $x$
    \begin{align*}
      \int \frac{y'(x)}{y(x)^2} \d x &= \int x \d x,\\
      \frac{-1}{y(x)} &= \answer[given]{\frac{x^2}{2}}+C
    \end{align*}
    and solve for $y(x)$ to find
    \[
    y(x) = \answer[given]{\frac{-1}{\frac{x^2}{2}+C}}.
    \]
    Since $y(0) =5$ we write
    \begin{align*}
    5&= y(0)\\
    &=\frac{-1}{C}
    \end{align*}
    So $C= -1/5$. Our final answer is
    \[
    y(x) = \frac{-1}{\frac{x^2}{2} \answer[given]{-\frac{1}{5}}}.
    \]
  \end{explanation}
\end{example}

Now that we've seen an example, let's give discuss this in general.

\begin{definition}
  A \dfn{separable differential equation} is a differential equation
  which can be written in the form
  \[
  G(y) y' = H(x)
  \]
  In other words, the independent variable $x$ and the function $y$
  can be placed on \textbf{separate} sides of the equals sign.
\end{definition}

\begin{warning}
  Calculus has lots of different notation. Each of these expressions
  means exactly the same thing:
  \begin{itemize}
  \item $y' = r\cdot y(1-y)$
  \item $y'(x) = r\cdot y(x)(1-y(x))$
  \item $\dd[y]{x} = r \cdot y(1-y)$
  \item $\dd{x} y(x) = r\cdot y(x) (1-y(x))$
  \end{itemize}
  We will work with all the notation above.
\end{warning}

\begin{question}
  Which of the following are separable differential equations?  Select all that apply.
  \begin{selectAll}
    \choice[correct]{$y' = y/x$}
    \choice{$y' = \sqrt{x^2+y^2}$}
    \choice[correct]{$\cos(y(x))y'(x) = \frac{x}{1+y(x)}$}
    \choice[correct]{$\dd[y]{x} = y+5$}
    \choice{$y'(x) = \sin(x+y(x))$}
    \choice{$\dd[y]{x} + x^2 y= x$}
    \choice{$\dd{x} y(x) = \sin(x) y(x) - \cos(x)$}
    \choice[correct]{$\dd{x} y(x) = -5 y(x)^{1/3}$}
  \end{selectAll}
  \begin{hint}
    To be a separable differential equation, we must collect $y$ and
    $y'$ on one side, and $x$ on the other. Typically, you will do
    this with multiplication or division.
  \end{hint}
\end{question}

The reason we care about separable differential equations is that:
\begin{enumerate}
\item Separable differential equations help model many real-world contexts.
\item Separable differential equations are solvable by humans.
\end{enumerate}
The basic ideas is if
\[
g(y)y' = H(x)
\]
then we can integrate both sides, writing
\begin{align*}
  G(y)y'  &= H(x)\\
  \int G(y) y' \d x &= \int H(x) \d x\\
  \int G(y) \d y &= \int H(x) \d x
\end{align*}
If we can symbolically compute these integrals, then we can solve for
$y$.



\begin{example}
  Suppose that 
  \begin{align*}
    g(y)y'  &= h(x)\\
    \int g(y) y' \d x &= \int h(x) \d x\\
    \int g(y) \d y &= \int h(x) \d x
  \end{align*}
  Let's see this strategy in action, and try to solve the differential equation $y' = \frac{x}{y^2}$.
  Write with me:
  First we separate the variables
  \[
  \answer{y^2} y' = \answer{x}
  \]
  
  Then we integrate both sides with respect to $x$
  
  \begin{align*}
    \int y^2 y' \d x &= \int x \d x\\
    \int y^2 \d y &= \int x \d x\\
    \answer{\frac{1}{3} y^3} &= \answer{\frac{1}{2}x^2}+C\\
    y &= \sqrt[3]{\answer{\frac{3}{2}x^2}+3C}
  \end{align*}
  
  Since $3C$ could be any constant we like, we can rewrite the general solution to this differential equation as 
  
  \[
  y = \sqrt[3]{\frac{3}{2}x^2+C}
  \]
  
  We can check that all of these functions really are solutions to the differential equation:
  
  \begin{align*}
    \frac{\d y}{\d x} &= \ddx \sqrt[3]{\frac{3}{2}x^2+C}\\
    &=(\frac{3}{2}x^2+C)^{-\frac{2}{3}} x\\
    &= \frac{x}{(\sqrt[3]{\frac{3}{2}x^2+C})^2}\\
    &= \frac{x}{y^2}
  \end{align*}
\end{example}


In the last example, it worked out that we could solve for $y$ as a function of $x$.  This is not always the case.

\begin{example}
  Consider the separable differential equation
  \[
  \cos(y) y' = x
  \]
  Integrating both sides yields
  \begin{align*}
    \int \cos(y) y' \d x = \int x \d x\\
    \int \cos(y) \d y = \int x \d x\\
    \sin(y) = \frac{1}{2}x^2+C
  \end{align*}
  This shows that any function satisfying the differential equation
  must satisfy this relation.  We call such a relation that a solution
  to a differential equation must satisfy a \dfn{implicit solution of a differential equation}.	
\end{example}

\begin{example}	
One really important example of a separable differential equation is
the \dfn{logistic equation}:
\[
y' = ry(1-y)
\]
This equation comes up frequently in population modeling.  

\begin{question}
  Which of the following are equilibrium solutions to this differential equation?
  \begin{multipleChoice}
    \choice[correct]{$y = 0$}
    \choice{$y = r$}
    \choice[correct]{$y = 1$}
  \end{multipleChoice}
\end{question}
Let us solve this equation together.  First we separate the differential equation:
\[
\answer{\frac{1}{y(1-y)}} y'  = r
\]
Now we integrate both sides with respect to $x$
\[
\int \frac{1}{y(1-y)} y' \d x =\int r \d x
\]
now using variable substitution we get
\[
\int \answer{\frac{1}{y(1-y)}} \d y = \int r \d x
\]
We need to use partial fraction decomposition to solve this integral.
We have
\[
\frac{1}{y(1-y)} = \frac{\answer{1}}{y}+\frac{\answer{1}}{1-y}
\]
So we get
\[
\int \frac{1}{y} + \frac{1}{1-y} \d y = \int r \d x
\]
This yields
\[
\ln(|y|) -  \ln(|1-y|)  = rx+C_1
\]
Now we can solve for $y$:
\begin{align*}
\ln(|y|) -  \ln(|1-y|)  &= rx+C_1\\
\ln(|\frac{y}{1-y}|) &= rx+C_1\\
|\frac{y}{1-y}| &= e^{rx+C_1}\\
\end{align*}
At this point, we can write $e^{rx+C_1} = e^{C_1} e^{rx}$.  We get $\frac{y}{1-y} = \pm e^{C_1} e^{rx}$.  If we rename $\pm e^{C_1}$ to be $C_2$, then we get
\begin{align*}
  \frac{y}{1-y} &=  C_2e^{rx}\\
  \frac{1-y}{y} &= C_3e^{-rx} \textrm{ where $C_3  =\frac{1}{C_2}$}\\
  \frac{1}{y} &= 1+C_3e^{-rx}\\
  y &= \frac{1}{1+C_3e^{-rx}}
\end{align*}
So this is the general solution to the logistic equation!
\end{example}





\end{document}
